Finished infrastructure - found bug! :)

dsss17/TImp.v
@@ -13,274 +13,504 @@ Import QcDefaultNotation. Open Scope qc_scope.
 
 (* /IMPORTS *)
 
-(* Maps as functions are bad, explicit maps instead *)
+(* TODO: This should be imported *)
+(** ** ATOM *)
 
-(* TODO: Put these back in QC? *)
+Require Import Equalities.
+Module Type ATOM <: UsualDecidableType.
 
-Inductive id : Type :=
-  | Id : string -> id.
+  Parameter t : Set.
+  Parameter eq_dec : forall (x y:t), {x = y} + {x <> y}.
+  Parameter fresh : list t -> t.
+  Parameter fresh_not_in : forall l, ~ In (fresh l) l.
+  Parameter nat_of: t -> nat.
 
-Derive (Arbitrary, Show) for id.
+  Include HasUsualEq <+ UsualIsEq.
 
-Instance eq_dec_id (x y : id) : Dec (x = y).
-constructor. unfold ssrbool.decidable. repeat decide equality. Defined.
+End ATOM.
 
-Definition beq_id x y :=
-  match x,y with
-    | Id n1, Id n2 => if string_dec n1 n2 then true else false
+(** ** Atom *)
+(** Implements the [ATOM] signature. *)
+
+Module Atom : ATOM.
+
+  Definition t := nat.
+  Definition eq_dec := eq_nat_dec.
+  
+  Fixpoint max_elt (al:list t) : t :=
+    match al with
+      | nil => 0
+      | n'::al' => max n' (max_elt al')
+    end.
+
+  Definition fresh (al:list t) : t :=
+    S (max_elt al).
+
+  Lemma max_elt_spec : forall al b,
+    In b al -> b <= max_elt al.
+(* FOLD *)
+  Proof.
+    intros. induction al. inversion H.
+      inversion H; subst; simpl. apply Nat.le_max_l.
+      eapply le_trans; auto with arith. (* apply Nat.le_max_r. *)
+  Qed.
+(* /FOLD *)
+    
+  Lemma fresh_not_in : forall l, 
+    ~ In (fresh l) l.
+(* FOLD *)
+  Proof.
+    unfold fresh, not. intros l Hin.
+    specialize (max_elt_spec _ _ Hin). intro Ha.
+    contradict Ha; apply le_Sn_n.
+  Qed.
+(* /FOLD *)
+
+  Include HasUsualEq <+ UsualIsEq.
+
+  Definition nat_of (a : nat) := a.
+  
+End Atom.
+
+(* Automatically unfold Atom.eq *)
+Global Arguments Atom.eq /.
+
+Instance show_atom : Show Atom.t :=
+  {| show x := show (Atom.nat_of x) |}.
+
+Fixpoint get_fresh_atoms n l :=
+  match n with
+  | 0 => l
+  | S n' => get_fresh_atoms n' ((Atom.fresh l) :: l)
   end.
 
-Theorem beq_id_refl : forall id, true = beq_id id id.
-Admitted. (* QuickChick beq_id_refl. *) 
+Definition fresh_store : list Atom.t := get_fresh_atoms 100 [].
+Definition gen_fresh (atom_store : list Atom.t) : G Atom.t := 
+  oneof (returnGen (Atom.fresh [])) (List.map returnGen atom_store).
 
-Theorem beq_id_true_iff : forall x y : id,
-  beq_id x y = true <-> x = y.
-Admitted. (* Prop *)
+Fixpoint index_of_atom_in_list (a : Atom.t) (l : list Atom.t) : option nat :=
+  match l with
+  | [] => None
+  | (a' :: l') => if Atom.eq_dec a a' then Some 0 else
+                   match index_of_atom_in_list a l' with
+                   | Some n => Some (S n)
+                   | None => None
+                   end
+  end.
+(* All of the above should be imported *)
 
-Theorem beq_id_false_iff : forall x y : id,
-  beq_id x y = false
-  <-> x <> y.
-Admitted. (* Prop *)
+Module Type Map (K:UsualDecidableType).
 
-Theorem false_beq_id : forall x y : id,
-   x <> y
-   -> beq_id x y = false.
-Admitted. (* QuickChick false_beq_id. *)
+Section withv.
+Variable V : Type.
 
-Definition partial_map := list (id * value).
+Parameter t : Type -> Type.
+Parameter empty : t V.
+Parameter get : t V -> K.t -> option V.
+Parameter set : t V -> K.t -> V -> t V.
+Parameter rem : t V -> K.t -> t V.
+Parameter dom : t V -> list K.t.
+Parameter forallb2 : (K.t -> V -> bool) -> t V -> bool.
 
-Definition empty : partial_map := nil.
 
-Definition update := @cons (id * value).
+Axiom update_eq : forall v k1 k2 m, k2 = k1 -> get (set m k1 v) k2 = Some v.
+Axiom update_neq : forall v k1 k2 m, k2 <> k1 -> get (set m k1 v) k2 = get m k2.
+Axiom get_in_dom : forall m k v, get m k = Some v -> In k (dom m).
+Axiom dom_in_get : forall m k, In k (dom m) -> exists v, get m k = Some v.
+Axiom get_forallb2 : forall m f,
+                       (forall k v, get m k = Some v -> f k v = true) 
+                       <-> forallb2 f m = true.
+End withv.
 
-Inductive bind : partial_map -> id -> value -> Prop :=
-  | BindNow   : forall x a m, bind (cons (x, a) m) x a
-  | BindLater : forall x x' a a' m',
-                  ~ (x = x') ->
-                  bind m' x a -> 
-                  bind (cons (x',a') m') x a.
+End Map.
 
-(* DELETE -- write by hand *)
-Derive ArbitrarySizedSuchThat for (fun x => bind m x a).
 
-(* NOT NEEDED
-Instance adm_st m a : SuchThatCorrect (fun x => bind m x a) (genST (fun x => bind m x a)).
-Admitted.
+Module ListMap (K:UsualDecidableType) <: Map K.
+
+Section withv.
+Context {V : Type}.
+
+Definition t := list (K.t * V).
+
+Definition empty : t := [].
+
+Fixpoint get m k : option V := 
+  match m with
+    | [] => None
+    | (k', v) :: m' => if K.eq_dec k k'
+                       then Some v
+                       else get m' k
+  end.
+
+Definition set (m:t) (k:K.t) (v:V) : t :=
+  (k, v) :: m.
+
+
+Fixpoint rem (m:t) (k:K.t) : t :=
+  match m with
+    | [] => []
+    | (k', v) :: m' => if K.eq_dec k k'
+                       then rem m' k
+                       else (k', v) :: rem m' k
+  end.
+
+Fixpoint dom (m:t) : list K.t :=
+  match m with
+    | [] => []
+    | (k', v) :: m' => k' :: dom m'
+  end.
+
+Fixpoint forallb2' (f:K.t -> V -> bool) (m:t) (d:list K.t) : bool :=
+     match d with
+       | [] => true
+       | k :: d' => match get m k with
+                      | None => false
+                      | Some v => f k v && forallb2' f m d'
+                    end
+     end.  
+
+Definition forallb2 (f:K.t -> V -> bool) (m:t) : bool :=
+  forallb2' f m (dom m).
+
+
+Lemma update_eq : forall v k1 k2 m,
+
+    k2 = k1 -> get (set m k1 v) k2 = Some v.
+Proof.
+  intros; simpl. destruct (K.eq_dec _ _); intuition.
+Qed.
+
+
+Lemma update_neq : forall v k1 k2 m,
+  k2 <> k1 -> get (set m k1 v) k2 = get m k2.
+Proof.
+  intros; simpl. destruct (K.eq_dec _ _); intuition.
+Qed.
+
+Lemma get_in_dom : forall m k v,
+  get m k = Some v -> In k (dom m).
+Proof.
+  induction m; intros k v. inversion 1.
+  destruct a as [k' v']; simpl in *. intros. destruct (K.eq_dec k k'); intuition eauto. 
+Qed.
+
+Lemma dom_in_get : forall m k,
+  In k (dom m) -> exists v, get m k = Some v.
+Proof.
+  induction m. inversion 1.
+  destruct a as [k' v']; simpl in *. 
+  intro k. destruct (K.eq_dec k k') as [|Heq]; intros. intuition eauto.
+  inversion H; eauto; contradict Heq; auto.
+Qed.
+
+Lemma get_forallb2' : forall m f P,
+  (forall k v, P k v <-> f k v = true) ->
+  ((forall k v, get m k = Some v -> P k v)
+   <-> forallb2 f m = true).
+Proof.
+  intros until 0. intro Hpf. unfold forallb2.
+  split; intros.
+
+  - (* Case "->". *)
+  pose proof (dom_in_get m) as Hd.
+  set (d := dom m) in *. clearbody d.
+
+  induction d. reflexivity. simpl. 
+  destruct (get m a) eqn:Hget.
+  rewrite IHd; auto. assert (f a v = true).
+  apply Hpf. eapply H; eauto. rewrite H0. simpl. reflexivity.
+  intros. apply Hd. simpl. right. auto.
+  
+  ecase (Hd a) as [v Hv]; try (left; auto). 
+  rewrite Hv in Hget. inversion Hget.
+
+  - (* Case "<-". *)
+  pose proof (get_in_dom m _ _ H0) as Hd.
+  set (d:=dom m) in *. clearbody d.
+
+  induction d. inversion Hd.
+  simpl in H.
+  destruct (K.eq_dec a k). subst a. rewrite H0 in H.
+  apply Hpf; auto. destruct (f k v); auto. 
+  apply IHd. destruct (get m a); try solve [inversion H].
+  destruct (f a v0).
+  destruct (forallb2' f m d); auto.
+  destruct (forallb2' f m d); auto.
+  inversion Hd; intuition.
+Qed.  
+
+Lemma get_forallb2 : forall m f,
+  (forall k v, get m k = Some v -> f k v = true) 
+  <-> 
+  forallb2 f m = true.
+Proof.
+  intros. unfold forallb2.
+  split; intros.
+
+  - (* Case "->". *)
+  pose proof (dom_in_get m) as Hd.
+  set (d := dom m) in *. clearbody d.
+
+  induction d. reflexivity. simpl. 
+  destruct (get m a) eqn:Hget.
+  rewrite H; auto. rewrite IHd; auto. intros.
+  apply Hd. simpl. right; auto.
+  
+  ecase (Hd a) as [v Hv]; try (left; auto). 
+  rewrite Hv in Hget. inversion Hget.
+
+  - (* Case "<-". *)
+  pose proof (get_in_dom m _ _ H0) as Hd.
+  set (d:=dom m) in *. clearbody d.
+
+  induction d. inversion Hd.
+  simpl in H.
+  destruct (K.eq_dec a k). subst a. rewrite H0 in H.
+  destruct (f k v); auto.
+  apply IHd.
+  destruct (get m a); try solve [inversion H].
+  destruct (forallb2' f m d); auto.
+  destruct (f a v0); auto.
+  inversion Hd; intuition.
+Qed.  
+
+End withv.
+
+End ListMap.
+
+
+
+(*
+Module Atom_as_OT : UsualOrderedType.
+  Definition t := Atom.t.
+  Definition eq := @eq t.
+
+  Definition eq_refl  := @eq_refl t.
+  Definition eq_sym   := @eq_sym t.
+  Definition eq_trans := @eq_trans t.
+
+  Definition lt a1 a2 := lt (Atom.nat_of a1) (Atom.nat_of a2).
+
+  Theorem lt_trans (a1 a2 a3: t) : lt a1 a2 -> lt a2 a3 -> lt a1 a3. Admitted.
+  Theorem lt_not_eq : forall x y : t, lt x y -> ~ eq x y. Admitted.
+  Definition compare : forall x y : t, Compare lt eq x y. Admitted.
+  Definition eq_dec : forall x y : t, {eq x y} + {~ eq x y}. Admitted.
+End Atom_as_OT.
+
+(* Alias - needed? *)
+Definition id := Atom_as_OT.t.
+
+Instance eq_dec_id (x y : id) : Dec (x = y) := 
+  { dec := Atom_as_OT.eq_dec x y }.
+
+(* Generators for Coq Library Maps *)
+Module Map := FMapList.Make(Atom_as_OT).
+
+(* Restrict a valuation to a set of unknowns *)
+Module MapProp := FMapFacts.Properties Map.
+Module MapFacts := FMapFacts.Facts Map.
 *)
 
-(* MOVE TO QC *)
-Instance checkFalse : Checkable False := {| checker := fun _ => checker false |}.
+(* Types *)
 
-Instance bind_dec m x v : Dec (bind m x v) :=
-  {| dec := _ |}.
-(* remove ssr...
-Proof.
-  move: x v.
-  induction m => x v.
-  - right => contra. inversion contra.
-  - destruct a as [x' v'].
-    destruct (eq_dec_id x x') as [[Eq | Neq]].
-    + destruct (Dec_eq_nat v v') as [[EqV | NeqV]].
-      * subst; left ; constructor; eauto.
-      * subst; right => Contra.
-        inversion Contra; subst; eauto.
-    + subst; specialize (IHm x v).
-      destruct IHm as [L | R].
-      * left; constructor; eauto.
-      * right => Contra; inversion Contra; subst; eauto.
+Inductive ty := TBool | TNat. 
+
+(* TODO: Actual Generators? *)
+Derive (Arbitrary, Show) for ty.
+Instance eq_dec_ty (x y : ty) : Dec (x = y).
+constructor; unfold ssrbool.decidable; decide equality.
 Defined.
-*) Admitted.
 
-(* TODO: Correct equivalence of maps *)
-Definition equiv_map m1 m2 :=
-  forall x v , bind m1 x v <-> bind m2 x v.
+Module AtomMap := ListMap (Atom).
 
-Conjecture apply_empty : forall x a, ~ (bind empty x a).
-(* QuickChick apply_empty. *)
-(* Gave Up! - QuickChick apply_empty_unfolded. *)
+Definition context := @AtomMap.t ty.
 
-Conjecture update_eq : forall (m: partial_map) x v,
-    bind (update (x,v) m) x v.
-(* QuickChick update_eq. *)
 
-(* TODO: Change it to equivalence === -- use Equivalence
-   typeclass?  (These are sadly false at the moment) *)
+(* Too many sigs *)
+Definition gen_context (n : nat) : G context := 
+  let domain := get_fresh_atoms n [] in
+  bindGen (vectorOf n arbitrary) (fun (range : list ty) => 
+  returnGen (List.fold_left (fun (m : context) (kv : Atom.t * ty) => 
+                               let (k,v) := kv in 
+                               AtomMap.set m k v) 
+                            (List.combine domain range) AtomMap.empty)).
 
-Theorem update_neq : forall v x1 x2
-                       (m : partial_map),
-  x2 <> x1 ->
-    forall v' v'', bind (cons (x2, v) m) x1 v' ->
-                   bind m x1 v'' ->
-                   v' = v''.
-Admitted. (* Leo: TODO QuickChick update_neq. *)
 
-Lemma update_shadow : forall (m: partial_map) v1 v2 x,
-  update (x, v2) (update (x, v1) m)  = update (x, v2) m.
-Admitted. (* QuickChick update_shadow. *)
+Definition gen_typed_atom_from_context (Gamma : context) (T : ty) : G (option Atom.t) :=
+  oneof (returnGen None) (List.map (fun aT' => returnGen (Some (fst aT'))) 
+                                   (List.filter (fun aT' => T = (snd aT')?) Gamma)).
 
-Theorem update_same : forall v x (m : partial_map),
-  bind m x v ->
-  update (x, v) m = m.
-Admitted. (* QuickChick update_same. *)
+(* Expressions *)
 
-Theorem update_permute : forall v1 v2 x1 x2
-                                (m : partial_map),
-  x2 <> x1 ->
-    (update (x1,v1) (update (x2,v2) m))
-  = (update (x2,v2) (update (x1,v1) m)).
-Admitted. (* QuickChick update_permute. *)
+Inductive exp : Type :=
+  | EVar : Atom.t -> exp
+  | ENum : nat -> exp
+  | EPlus : exp -> exp -> exp
+  | EMinus : exp -> exp -> exp
+  | EMult : exp -> exp -> exp
+  | ETrue : exp
+  | EFalse : exp
+  | EEq : exp -> exp -> exp
+  | ELe : exp -> exp -> exp
+  | ENot : exp -> exp
+  | EAnd : exp -> exp -> exp.
+
+(* For automatic, get must be inductive *)
+Inductive has_type : context -> exp -> ty -> Prop := 
+| Ty_Var : forall x T Gamma, AtomMap.get Gamma x = Some T -> has_type Gamma (EVar x) T
+| Ty_Num : forall Gamma n, has_type Gamma (ENum n) TNat
+| Ty_Plus : forall Gamma e1 e2, has_type Gamma e1 TNat -> has_type Gamma e2 TNat ->
+                                has_type Gamma (EPlus e1 e2) TNat
+| Ty_Minus : forall Gamma e1 e2, has_type Gamma e1 TNat -> has_type Gamma e2 TNat ->
+                                has_type Gamma (EMinus e1 e2) TNat
+| Ty_Mult : forall Gamma e1 e2, has_type Gamma e1 TNat -> has_type Gamma e2 TNat ->
+                                has_type Gamma (EMult e1 e2) TNat
+| Ty_True : forall Gamma, has_type Gamma ETrue TBool
+| Ty_False : forall Gamma, has_type Gamma EFalse TBool
+| Ty_Eq : forall Gamma e1 e2, has_type Gamma e1 TNat -> has_type Gamma e2 TNat ->
+                              has_type Gamma (EEq e1 e2) TBool
+| Ty_Le : forall Gamma e1 e2, has_type Gamma e1 TNat -> has_type Gamma e2 TNat ->
+                              has_type Gamma (ELe e1 e2) TBool
+| Ty_Not : forall Gamma e, has_type Gamma e TBool ->
+                              has_type Gamma (ENot e) TBool
+| Ty_And : forall Gamma e1 e2, has_type Gamma e1 TBool -> has_type Gamma e2 TBool ->
+                               has_type Gamma (EAnd e1 e2) TBool.
+
+Import QcDoNotation.
+(* This is so pedantic I want to derive it :) *)
+Fixpoint gen_exp_typed_sized (size : nat) (Gamma : context) (T : ty) : G (option exp) :=
+  let gen_typed_evar := 
+      doM! x <- gen_typed_atom_from_context Gamma T;
+        returnGen (Some (EVar x)) in
+  let base :=
+      match T with 
+      | TNat  => [ (2, do! n <- arbitrary; returnGen (Some (ENum n)))]
+      | TBool => [ (1, returnGen (Some ETrue))
+                 ; (1, returnGen (Some EFalse)) ]
+      end in 
+  let recs size' := 
+      match T with 
+      | TNat => [ (1, doM! e1 <- gen_exp_typed_sized size' Gamma TNat; 
+                      doM! e2 <- gen_exp_typed_sized size' Gamma TNat; 
+                      returnGen (Some (EPlus e1 e2))) 
+                ; (1, doM! e1 <- gen_exp_typed_sized size' Gamma TNat; 
+                      doM! e2 <- gen_exp_typed_sized size' Gamma TNat; 
+                      returnGen (Some (EMinus e1 e2))) 
+                ; (1, doM! e1 <- gen_exp_typed_sized size' Gamma TNat; 
+                      doM! e2 <- gen_exp_typed_sized size' Gamma TNat; 
+                      returnGen (Some (EMult e1 e2))) ]
+      | TBool => [ (1, doM! e1 <- gen_exp_typed_sized size' Gamma TNat; 
+                       doM! e2 <- gen_exp_typed_sized size' Gamma TNat; 
+                       returnGen (Some (EEq e1 e2))) 
+                 ; (1, doM! e1 <- gen_exp_typed_sized size' Gamma TNat; 
+                       doM! e2 <- gen_exp_typed_sized size' Gamma TNat; 
+                       returnGen (Some (ELe e1 e2))) 
+                 ; (1, doM! e1 <- gen_exp_typed_sized size' Gamma TBool; 
+                       returnGen (Some (ENot e1)))
+                 ; (1, doM! e1 <- gen_exp_typed_sized size' Gamma TBool; 
+                       doM! e2 <- gen_exp_typed_sized size' Gamma TBool; 
+                       returnGen (Some (EAnd e1 e2))) ]
+      end in
+  match size with 
+  | O => 
+    freq ( (1, gen_typed_evar) ;; base )
+  | S size' => 
+    freq ( (1, gen_typed_evar) ;; (base ++ recs size'))
+  end.
 
 Inductive value := VNat : nat -> value | VBool : bool -> value.
 
-(* ################################################################# *)
-(** * Arithmetic and Boolean Expressions *)
+Derive Show for value.
+  
+Inductive has_type_value : value -> ty -> Prop :=
+  | TyVNat  : forall n, has_type_value (VNat  n) TNat
+  | TyVBool : forall b, has_type_value (VBool b) TBool.
 
-(** We'll present Imp in three parts: first a core language of
-    _arithmetic and boolean expressions_, then an extension of these
-    expressions with _variables_, and finally a language of _commands_
-    including assignment, conditions, sequencing, and loops. *)
-
-(* ================================================================= *)
-(** ** Syntax *)
-
-Module AExp.
-
-(** These two definitions specify the _abstract syntax_ of
-    arithmetic and boolean expressions. *)
-
-Inductive exp : Type :=
-  | Var : id -> exp
-  | ANum : nat -> exp
-  | APlus : exp -> exp -> exp
-  | AMinus : exp -> exp -> exp
-  | AMult : exp -> exp -> exp
-  | BTrue : exp
-  | BFalse : exp
-  | BEq : exp -> exp -> exp
-  | BLe : exp -> exp -> exp
-  | BNot : exp -> exp
-  | BAnd : exp -> exp -> exp.
-
-Definition state := partial_map nat.
-
-Definition empty_state : state :=
-  t_empty 0.
-
-(* ================================================================= *)
-(** ** Syntax  *)
-
-(** We can add variables to the arithmetic expressions we had before by
-    simply adding one more constructor: *)
-
-Inductive exp : Type :=
-  | ANum : nat -> exp
-  | AId : id -> exp                (* <----- NEW *)
-  | APlus : exp -> exp -> exp
-  | AMinus : exp -> exp -> exp
-  | AMult : exp -> exp -> exp.
-
-(** Defining a few variable names as notational shorthands will make
-    examples easier to read: *)
-
-Definition W : id := Id "W".
-Definition X : id := Id "X".
-Definition Y : id := Id "Y".
-Definition Z : id := Id "Z".
-
-(** (This convention for naming program variables ([X], [Y],
-    [Z]) clashes a bit with our earlier use of uppercase letters for
-    types.  Since we're not using polymorphism heavily in the chapters
-    devoped to Imp, this overloading should not cause confusion.) *)
-
-(** The definition of [exp]s is unchanged (except for using the new
-    [exp]s): *)
-
-Inductive exp : Type :=
-  | BTrue : exp
-  | BFalse : exp
-  | BEq : exp -> exp -> exp
-  | BLe : exp -> exp -> exp
-  | BNot : exp -> exp
-  | BAnd : exp -> exp -> exp.
-
-(* ================================================================= *)
-(** ** Evaluation *)
-
-(** The arith and boolean evaluators are extended to handle
-    variables in the obvious way, taking a state as an extra
-    argument: *)
-
-Fixpoint aeval (st : state) (a : exp) : nat :=
-  match a with
-  | ANum n => n
-  | AId x => st x                                (* <----- NEW *)
-  | APlus a1 a2 => (aeval st a1) + (aeval st a2)
-  | AMinus a1 a2  => (aeval st a1) - (aeval st a2)
-  | AMult a1 a2 => (aeval st a1) * (aeval st a2)
+Definition gen_typed_value (T : ty) : G value :=
+  match T with 
+  | TNat  => do! n <- arbitrary; returnGen (VNat n)
+  | TBool => do! b <- arbitrary; returnGen (VBool b)
   end.
 
-Fixpoint beval (st : state) (b : exp) : bool :=
-  match b with
-  | BTrue       => true
-  | BFalse      => false
-  | BEq a1 a2   => beq_nat (aeval st a1) (aeval st a2)
-  | BLe a1 a2   => leb (aeval st a1) (aeval st a2)
-  | BNot b1     => negb (beval st b1)
-  | BAnd b1 b2  => andb (beval st b1) (beval st b2)
+Definition state := @AtomMap.t value.
+
+(* For auto - change to inductive *)
+Inductive typed_state : context -> state -> Prop :=
+| Typed_State : forall Gamma st x v T, 
+    AtomMap.get Gamma x = Some T ->
+    AtomMap.get st x = Some v ->
+    has_type_value v T ->
+    typed_state Gamma st.
+
+Definition gen_typed_state (Gamma : context) : G state := 
+  sequenceGen (List.map (fun '(x, T) =>
+                           do! v <- gen_typed_value T; 
+                           returnGen (x, v)) Gamma).
+
+(* More monads? :/ *)
+(*
+Definition bindOption {A B : Type} (m : option A) (k : A -> option B) : option B :=
+  match m with 
+  | Some a => k a 
+  | _ => None 
   end.
-
-Example exp1 :
-  aeval (t_update empty_state X 5)
-        (APlus (ANum 3) (AMult (AId X) (ANum 2)))
-  = 13.
-Proof. reflexivity. Qed.
-
-Example exp1 :
-  beval (t_update empty_state X 5)
-        (BAnd BTrue (BNot (BLe (AId X) (ANum 4))))
-  = true.
-Proof. reflexivity. Qed.
-
-(* ################################################################# *)
-(** * Commands *)
-
-(** Now we are ready define the syntax and behavior of Imp
-    _commands_ (sometimes called _statements_). *)
-
-(* ================================================================= *)
-(** ** Syntax *)
-
-(** Informally, commands [c] are described by the following BNF
-    grammar.  (We choose this slightly awkward concrete syntax for the
-    sake of being able to define Imp syntax using Coq's Notation
-    mechanism.  In particular, we use [IFB] to avoid conflicting with
-    the [if] notation from the standard library.)
-
-     c ::= SKIP | x ::= a | c ;; c | IFB b THEN c ELSE c FI
-         | WHILE b DO c END
+Notation "'do!' X <- A ; B" :=
+  (bindOption A (fun X => B))
+  (at level 200, X ident, A at level 100, B at level 200).
 *)
-(**
-    For example, here's factorial in Imp:
 
-     Z ::= X;;
-     Y ::= 1;;
-     WHILE not (Z = 0) DO
-       Y ::= Y * Z;;
-       Z ::= Z - 1
-     END
-
-   When this command terminates, the variable [Y] will contain the
-   factorial of the initial value of [X]. *)
-
-(** Here is the formal definition of the abstract syntax of
-    commands: *)
+Fixpoint eval (st : state) (e : exp) : option value :=
+  match e with
+  | EVar x => AtomMap.get st x
+  | ENum n => Some (VNat n)
+  | EPlus e1 e2 => 
+    match eval st e1, eval st e2 with 
+    | Some (VNat n1), Some (VNat n2) => Some (VNat (n1 + n2))
+    | _, _ => None
+    end
+  | EMinus e1 e2 => 
+    match eval st e1, eval st e2 with 
+    | Some (VNat n1), Some (VNat n2) => Some (VNat (n1 - n2))
+    | _, _ => None
+    end
+  | EMult e1 e2 => 
+    match eval st e1, eval st e2 with 
+    | Some (VNat n1), Some (VNat n2) => Some (VNat (n1 * n2))
+    | _, _ => None
+    end
+  | ETrue       => Some (VBool true  )
+  | EFalse      => Some (VBool false )
+  | EEq e1 e2 => 
+    match eval st e1, eval st e2 with 
+    | Some (VNat n1), Some (VNat n2) => Some (VBool (n1 =? n2))
+    | _, _ => None
+    end
+  | ELe e1 e2 => 
+    match eval st e1, eval st e2 with 
+    | Some (VNat n1), Some (VNat n2) => Some (VBool (n1 <? n2))
+    | _, _ => None
+    end
+  | ENot e => 
+    match eval st e with 
+    | Some (VBool b) => Some (VBool (negb b))
+    | _ => None
+    end
+  | EAnd e1 e2  => 
+    match eval st e1, eval st e2 with 
+    | Some (VBool b1), Some (VBool b2) => Some (VBool (andb b1 b2))
+    | _, _ => None
+    end
+  end.
 
 Inductive com : Type :=
-  | CSkip : com
-  | CAss : id -> exp -> com
-  | CSeq : com -> com -> com
-  | CIf : exp -> com -> com -> com
-  | CWhile : exp -> com -> com.
+  | CSkip  : com
+  | CAss   : Atom.t -> exp -> com
+  | CSeq   : com    -> com -> com
+  | CIf    : exp    -> com -> com -> com
+  | CWhile : exp    -> com -> com.
+
+Derive Show for exp.
+Derive Show for com.
 
 (** As usual, we can use a few [Notation] declarations to make things
     more readable.  To avoid conflicts with Coq's built-in notations,
@@ -299,84 +529,94 @@ Notation "'WHILE' b 'DO' c 'END'" :=
 Notation "'IFB' c1 'THEN' c2 'ELSE' c3 'FI'" :=
   (CIf c1 c2 c3) (at level 80, right associativity).
 
-(** For example, here is the factorial function again, written as a
-    formal definition to Coq: *)
-
-Definition fact_in_coq : com :=
-  Z ::= AId X;;
-  Y ::= ANum 1;;
-  WHILE BNot (BEq (AId Z) (ANum 0)) DO
-    Y ::= AMult (AId Y) (AId Z);;
-    Z ::= AMinus (AId Z) (ANum 1)
-  END.
-
-(* ================================================================= *)
-(** ** More Examples *)
-
-(** Assignment: *)
-
-Definition plus2 : com :=
-  X ::= (APlus (AId X) (ANum 2)).
-
-Definition XtimesYinZ : com :=
-  Z ::= (AMult (AId X) (AId Y)).
-
-Definition subtract_slowly_body : com :=
-  Z ::= AMinus (AId Z) (ANum 1) ;;
-  X ::= AMinus (AId X) (ANum 1).
-
-(* ----------------------------------------------------------------- *)
-(** *** Loops *)
-
-Definition subtract_slowly : com :=
-  WHILE BNot (BEq (AId X) (ANum 0)) DO
-    subtract_slowly_body
-  END.
-
-Definition subtract_3_from_5_slowly : com :=
-  X ::= ANum 3 ;;
-  Z ::= ANum 5 ;;
-  subtract_slowly.
-
-(* ----------------------------------------------------------------- *)
-(** *** An infinite loop: *)
-
-Definition loop : com :=
-  WHILE BTrue DO
-    SKIP
-  END.
-
-(* ################################################################# *)
-(** * Evaluating Commands *)
-
-(** Next we need to define what it means to evaluate an Imp command.
-    The fact that [WHILE] loops don't necessarily terminate makes defining
-    an evaluation function tricky... *)
-
-(* ================================================================= *)
-(** ** Evaluation as a Function (Failed Attempt) *)
-
-(** Here's an attempt at defining an evaluation function for commands,
-    omitting the [WHILE] case. *)
-
-Fixpoint ceval_fun_no_while (st : state) (c : com)
-                          : state :=
-  match c with
-    | SKIP =>
-        st
-    | x ::= a1 =>
-        t_update st x (aeval st a1)
-    | c1 ;; c2 =>
-        let st' := ceval_fun_no_while st c1 in
-        ceval_fun_no_while st' c2
-    | IFB b THEN c1 ELSE c2 FI =>
-        if (beval st b)
-          then ceval_fun_no_while st c1
-          else ceval_fun_no_while st c2
-    | WHILE b DO c END =>
-        st  (* bogus *)
+(* This is so pedantic I want to derive it :) *)
+Fixpoint gen_com_typed_sized (size : nat) (Gamma : context) : G (option com) :=
+  let assgn := 
+                (List.map (fun '(x,T) =>
+                             (1, doM! e <- gen_exp_typed_sized size Gamma T;
+                                returnGen (Some (CAss x e))))
+                          Gamma)
+  in 
+  let skip :=
+      returnGen (Some SKIP) in
+  let recs size' := 
+      [ (1, doM! c1 <- gen_com_typed_sized size' Gamma;
+            doM! c2 <- gen_com_typed_sized size' Gamma;
+            returnGen (Some (CSeq c1 c2))) 
+      ; (1, doM! c <- gen_com_typed_sized size' Gamma;
+            doM! b <- gen_exp_typed_sized size' Gamma TBool;
+            returnGen (Some (CWhile b c)))
+      ; (1, doM! b <- gen_exp_typed_sized size' Gamma TBool;
+            doM! c1 <- gen_com_typed_sized size' Gamma;
+            doM! c2 <- gen_com_typed_sized size' Gamma;
+            returnGen (Some (CIf b c1 c2)))
+      ] in
+  match size with 
+  | O => freq ((1, skip) ;; assgn)
+  | S size' => freq ((1, skip) ;; (assgn ++ recs size'))
   end.
 
+Inductive result := 
+| Success : state -> result
+| Fail : result 
+| OutOfGas : result. 
+
+(* State monad like fuel, or depth-like? *)
+Fixpoint ceval (fuel : nat) (st : state) (c : com) : result :=
+  match fuel with 
+  | O => OutOfGas
+  | S fuel' => 
+    match c with
+    | SKIP =>
+        Success st
+    | x ::= e =>
+        match eval st e with 
+        | Some v => Success (AtomMap.set st x v)
+        | _ => Fail 
+        end
+    | c1 ;; c2 =>
+        match ceval fuel' st c1 with 
+        | Success st' =>  ceval fuel' st' c2 
+        | _ => Fail
+        end
+    | IFB b THEN c1 ELSE c2 FI =>
+      match eval st b with 
+      | Some (VBool b) =>
+        ceval fuel' st (if b then c1 else c2)
+      | _ => Fail
+      end
+    | WHILE b DO c END =>
+      match eval st b with 
+      | Some (VBool b') =>
+        if b' then ceval fuel' st (c;; WHILE b DO c END) else Success st
+      | _ => Fail
+      end
+    end
+  end.
+
+Definition isFail r := 
+  match r with 
+  | Fail => true
+  | _ => false
+  end.
+
+Conjecture well_typed_state_never_stuck : 
+  forall Gamma st, typed_state Gamma st ->
+  forall fuel c, isFail (ceval fuel st c) = false.
+
+Definition well_typed_state_never_stuck := 
+  let num_vars := 4 in 
+  let top_level_size := 5 in
+  forAll (gen_context num_vars)  (fun Gamma =>
+  forAll (gen_typed_state Gamma) (fun st =>
+  forAll arbitrary (fun fuel =>
+  forAll gen_com_typed_sized  (fun c => 
+  negb (isFail (ceval fuel st c)))))).                      
+                          
+  
+
+
+(* LEO: Fix in SF: it should be c ;; WHILE ... (double ;) *)
 (** In a traditional functional programming language like OCaml or
     Haskell we could add the [WHILE] case as follows:
 
@@ -384,614 +624,9 @@ Fixpoint ceval_fun_no_while (st : state) (c : com)
     match c with
       ...
       | WHILE b DO c END =>
-          if (beval st b)
+          if (eval st b)
             then ceval_fun st (c; WHILE b DO c END)
             else st
     end.
-
-    Coq doesn't accept such a definition ("Error: Cannot guess
-    decreasing argument of fix") because the function we want to
-    define is not guaranteed to terminate. Indeed, it _doesn't_ always
-    terminate: for example, the full version of the [ceval_fun]
-    function applied to the [loop] program above would never
-    terminate. Since Coq is not just a functional programming
-    language but also a consistent logic, any potentially
-    non-terminating function needs to be rejected. Here is
-    an (invalid!) program showing what would go wrong if Coq
-    allowed non-terminating recursive functions:
-
-         Fixpoint loop_false (n : nat) : False := loop_false n.
-
-    That is, propositions like [False] would become provable
-    ([loop_false 0] would be a proof of [False]), which
-    would be a disaster for Coq's logical consistency.
-
-    Thus, because it doesn't terminate on all inputs,
-    of [ceval_fun] cannot be written in Coq -- at least not without
-    additional tricks and workarounds (see chapter [ImpCEvalFun]
-    if you're curious about what those might be). *)
-
-(* ================================================================= *)
-(** ** Evaluation as a Relation *)
-
-(** Here's a better way: define [ceval] as a _relation_ rather than a
-    _function_ -- i.e., define it in [Prop] instead of [Type], as we
-    did for [aevalR] above. *)
-
-(** This is an important change.  Besides freeing us from awkward
-    workarounds, it gives us a lot more flexibility in the definition.
-    For example, if we add nondeterministic features like [any] to the
-    language, we want the definition of evaluation to be
-    nondeterministic -- i.e., not only will it not be total, it will
-    not even be a function! *)
-
-(** We'll use the notation [c / st \\ st'] for the [ceval] relation:
-    [c / st \\ st'] means that executing program [c] in a starting
-    state [st] results in an ending state [st'].  This can be
-    pronounced "[c] takes state [st] to [st']". *)
-
-(* ----------------------------------------------------------------- *)
-(** *** Operational Semantics *)
-
-(** Here is an informal definition of evaluation, presented as inference
-    rules for readability:
-
-                           ----------------                            (E_Skip)
-                           SKIP / st \\ st
-
-                           aeval st a1 = n
-                   --------------------------------                     (E_Ass)
-                   x := a1 / st \\ (t_update st x n)
-
-                           c1 / st \\ st'
-                          c2 / st' \\ st''
-                         -------------------                            (E_Seq)
-                         c1;;c2 / st \\ st''
-
-                          beval st b1 = true
-                           c1 / st \\ st'
-                -------------------------------------                (E_IfTrue)
-                IF b1 THEN c1 ELSE c2 FI / st \\ st'
-
-                         beval st b1 = false
-                           c2 / st \\ st'
-                -------------------------------------               (E_IfFalse)
-                IF b1 THEN c1 ELSE c2 FI / st \\ st'
-
-                         beval st b = false
-                    ------------------------------               (E_WhileFalse)
-                    WHILE b DO c END / st \\ st
-
-                          beval st b = true
-                           c / st \\ st'
-                  WHILE b DO c END / st' \\ st''
-                  ---------------------------------               (E_WhileTrue)
-                    WHILE b DO c END / st \\ st''
 *)
-
-(** Here is the formal definition.  Make sure you understand
-    how it corresponds to the inference rules. *)
-
-Reserved Notation "c1 '/' st '\\' st'"
-                  (at level 40, st at level 39).
-
-Inductive ceval : com -> state -> state -> Prop :=
-  | E_Skip : forall st,
-      SKIP / st \\ st
-  | E_Ass  : forall st a1 n x,
-      aeval st a1 = n ->
-      (x ::= a1) / st \\ (t_update st x n)
-  | E_Seq : forall c1 c2 st st' st'',
-      c1 / st  \\ st' ->
-      c2 / st' \\ st'' ->
-      (c1 ;; c2) / st \\ st''
-  | E_IfTrue : forall st st' b c1 c2,
-      beval st b = true ->
-      c1 / st \\ st' ->
-      (IFB b THEN c1 ELSE c2 FI) / st \\ st'
-  | E_IfFalse : forall st st' b c1 c2,
-      beval st b = false ->
-      c2 / st \\ st' ->
-      (IFB b THEN c1 ELSE c2 FI) / st \\ st'
-  | E_WhileFalse : forall b st c,
-      beval st b = false ->
-      (WHILE b DO c END) / st \\ st
-  | E_WhileTrue : forall st st' st'' b c,
-      beval st b = true ->
-      c / st \\ st' ->
-      (WHILE b DO c END) / st' \\ st'' ->
-      (WHILE b DO c END) / st \\ st''
-
-  where "c1 '/' st '\\' st'" := (ceval c1 st st').
-
-(** The cost of defining evaluation as a relation instead of a
-    function is that we now need to construct _proofs_ that some
-    program evaluates to some result state, rather than just letting
-    Coq's computation mechanism do it for us. *)
-
-Example ceval_example1:
-    (X ::= ANum 2;;
-     IFB BLe (AId X) (ANum 1)
-       THEN Y ::= ANum 3
-       ELSE Z ::= ANum 4
-     FI)
-   / empty_state
-   \\ (t_update (t_update empty_state X 2) Z 4).
-Proof.
-  (* We must supply the intermediate state *)
-  apply E_Seq with (t_update empty_state X 2).
-  - (* assignment command *)
-    apply E_Ass. reflexivity.
-  - (* if command *)
-    apply E_IfFalse.
-      reflexivity.
-      apply E_Ass. reflexivity.  Qed.
-
-(** **** Exercise: 2 stars (ceval_example2)  *)
-Example ceval_example2:
-    (X ::= ANum 0;; Y ::= ANum 1;; Z ::= ANum 2) / empty_state \\
-    (t_update (t_update (t_update empty_state X 0) Y 1) Z 2).
-Proof.
-  (* FILL IN HERE *) Admitted.
-(** [] *)
-
-(** **** Exercise: 3 stars, advanced (pup_to_n)  *)
-(** Write an Imp program that sums the numbers from [1] to
-   [X] (inclusive: [1 + 2 + ... + X]) in the variable [Y].
-   Prove that this program executes as intended for [X] = [2]
-   (this is trickier than you might expect). *)
-
-Definition pup_to_n : com
-  (* REPLACE THIS LINE WITH ":= _your_definition_ ." *). Admitted.
-
-Theorem pup_to_2_ceval :
-  pup_to_n / (t_update empty_state X 2) \\
-    t_update (t_update (t_update (t_update (t_update (t_update empty_state
-      X 2) Y 0) Y 2) X 1) Y 3) X 0.
-Proof.
-  (* FILL IN HERE *) Admitted.
-(** [] *)
-
-(* ================================================================= *)
-(** ** Determinism of Evaluation *)
-
-(** Changing from a computational to a relational definition of
-    evaluation is a good move because it frees us from the artificial
-    requirement that evaluation should be a total function.  But it
-    also raises a question: Is the second definition of evaluation
-    really a partial function?  Or is it possible that, beginning from
-    the same state [st], we could evaluate some command [c] in
-    different ways to reach two different output states [st'] and
-    [st'']?
-
-    In fact, this cannot happen: [ceval] _is_ a partial function: *)
-
-Theorem ceval_deterministic: forall c st st1 st2,
-     c / st \\ st1  ->
-     c / st \\ st2 ->
-     st1 = st2.
-Proof.
-  intros c st st1 st2 E1 E2.
-  generalize dependent st2.
-  induction E1;
-           intros st2 E2; inversion E2; subst.
-  - (* E_Skip *) reflexivity.
-  - (* E_Ass *) reflexivity.
-  - (* E_Seq *)
-    assert (st' = st'0) as EQ1.
-    { (* Proof of assertion *) apply IHE1_1; assumption. }
-    subst st'0.
-    apply IHE1_2. assumption.
-  - (* E_IfTrue, b1 evaluates to true *)
-      apply IHE1. assumption.
-  - (* E_IfTrue,  b1 evaluates to false (contradiction) *)
-      rewrite H in H5. inversion H5.
-  - (* E_IfFalse, b1 evaluates to true (contradiction) *)
-    rewrite H in H5. inversion H5.
-  - (* E_IfFalse, b1 evaluates to false *)
-      apply IHE1. assumption.
-  - (* E_WhileFalse, b1 evaluates to false *)
-    reflexivity.
-  - (* E_WhileFalse, b1 evaluates to true (contradiction) *)
-    rewrite H in H2. inversion H2.
-  - (* E_WhileTrue, b1 evaluates to false (contradiction) *)
-    rewrite H in H4. inversion H4.
-  - (* E_WhileTrue, b1 evaluates to true *)
-      assert (st' = st'0) as EQ1.
-      { (* Proof of assertion *) apply IHE1_1; assumption. }
-      subst st'0.
-      apply IHE1_2. assumption.  Qed.
-
-(* ################################################################# *)
-(** * Reasoning About Imp Programs *)
-
-(** We'll get deeper into systematic techniques for reasoning about
-    Imp programs in the following chapters, but we can do quite a bit
-    just working with the bare definitions.  This section explores
-    some examples. *)
-
-Theorem plus2_spec : forall st n st',
-  st X = n ->
-  plus2 / st \\ st' ->
-  st' X = n + 2.
-Proof.
-  intros st n st' HX Heval.
-
-  (** Inverting [Heval] essentially forces Coq to expand one step of
-      the [ceval] computation -- in this case revealing that [st']
-      must be [st] extended with the new value of [X], since [plus2]
-      is an assignment *)
-
-  inversion Heval. subst. clear Heval. simpl.
-  apply t_update_eq.  Qed.
-
-(** **** Exercise: 3 stars, recommendedM (XtimesYinZ_spec)  *)
-(** State and prove a specification of [XtimesYinZ]. *)
-
-(* FILL IN HERE *)
-(** [] *)
-
-(** **** Exercise: 3 stars, recommended (loop_never_stops)  *)
-Theorem loop_never_stops : forall st st',
-  ~(loop / st \\ st').
-Proof.
-  intros st st' contra. unfold loop in contra.
-  remember (WHILE BTrue DO SKIP END) as loopdef
-           eqn:Heqloopdef.
-
-  (** Proceed by induction on the assumed derivation showing that
-      [loopdef] terminates.  Most of the cases are immediately
-      contradictory (and so can be solved in one step with
-      [inversion]). *)
-
-  (* FILL IN HERE *) Admitted.
-(** [] *)
-
-(** **** Exercise: 3 stars (no_whilesR)  *)
-(** Consider the following function: *)
-
-Fixpoint no_whiles (c : com) : bool :=
-  match c with
-  | SKIP =>
-      true
-  | _ ::= _ =>
-      true
-  | c1 ;; c2 =>
-      andb (no_whiles c1) (no_whiles c2)
-  | IFB _ THEN ct ELSE cf FI =>
-      andb (no_whiles ct) (no_whiles cf)
-  | WHILE _ DO _ END  =>
-      false
-  end.
-
-(** This predicate yields [true] just on programs that have no while
-    loops.  Using [Inductive], write a property [no_whilesR] such that
-    [no_whilesR c] is provable exactly when [c] is a program with no
-    while loops.  Then prove its equivalence with [no_whiles]. *)
-
-Inductive no_whilesR: com -> Prop :=
- (* FILL IN HERE *)
-.
-
-Theorem no_whiles_eqv:
-   forall c, no_whiles c = true <-> no_whilesR c.
-Proof.
-  (* FILL IN HERE *) Admitted.
-(** [] *)
-
-(** **** Exercise: 4 starsM (no_whiles_terminating)  *)
-(** Imp programs that don't involve while loops always terminate.
-    State and prove a theorem [no_whiles_terminating] that says this. *)
-(** Use either [no_whiles] or [no_whilesR], as you prefer. *)
-
-(* FILL IN HERE *)
-(** [] *)
-
-(* ################################################################# *)
-(** * Additional Exercises *)
-
-(** **** Exercise: 3 stars (stack_compiler)  *)
-(** HP Calculators, programming languages like Forth and Postscript
-    and abstract machines like the Java Virtual Machine all evaluate
-    arithmetic expressions using a stack. For instance, the expression
-
-      (2*3)+(3*(4-2))
-
-   would be entered as
-
-      2 3 * 3 4 2 - * +
-
-   and evaluated like this (where we show the program being evaluated
-   on the right and the contents of the stack on the left):
-
-      [ ]           |    2 3 * 3 4 2 - * +
-      [2]           |    3 * 3 4 2 - * +
-      [3, 2]        |    * 3 4 2 - * +
-      [6]           |    3 4 2 - * +
-      [3, 6]        |    4 2 - * +
-      [4, 3, 6]     |    2 - * +
-      [2, 4, 3, 6]  |    - * +
-      [2, 3, 6]     |    * +
-      [6, 6]        |    +
-      [12]          |
-
-  The task of this exercise is to write a small compiler that
-  translates [exp]s into stack machine instructions.
-
-  The instruction set for our stack language will consist of the
-  following instructions:
-     - [SPush n]: Push the number [n] on the stack.
-     - [SLoad x]: Load the identifier [x] from the store and push it
-                  on the stack
-     - [SPlus]:   Pop the two top numbers from the stack, add them, and
-                  push the result onto the stack.
-     - [SMinus]:  Similar, but subtract.
-     - [SMult]:   Similar, but multiply. *)
-
-Inductive sinstr : Type :=
-| SPush : nat -> sinstr
-| SLoad : id -> sinstr
-| SPlus : sinstr
-| SMinus : sinstr
-| SMult : sinstr.
-
-(** Write a function to evaluate programs in the stack language. It
-    should take as input a state, a stack represented as a list of
-    numbers (top stack item is the head of the list), and a program
-    represented as a list of instructions, and it should return the
-    stack after executing the program.  Test your function on the
-    examples below.
-
-    Note that the specification leaves unspecified what to do when
-    encountering an [SPlus], [SMinus], or [SMult] instruction if the
-    stack contains less than two elements.  In a sense, it is
-    immaterial what we do, since our compiler will never emit such a
-    malformed program. *)
-
-Fixpoint s_execute (st : state) (stack : list nat)
-                   (prog : list sinstr)
-                 : list nat
-  (* REPLACE THIS LINE WITH ":= _your_definition_ ." *). Admitted.
-
-Example s_execute1 :
-     s_execute empty_state []
-       [SPush 5; SPush 3; SPush 1; SMinus]
-   = [2; 5].
-(* FILL IN HERE *) Admitted.
-
-Example s_execute2 :
-     s_execute (t_update empty_state X 3) [3;4]
-       [SPush 4; SLoad X; SMult; SPlus]
-   = [15; 4].
-(* FILL IN HERE *) Admitted.
-
-(** Next, write a function that compiles an [exp] into a stack
-    machine program. The effect of running the program should be the
-    same as pushing the value of the expression on the stack. *)
-
-Fixpoint s_compile (e : exp) : list sinstr
-  (* REPLACE THIS LINE WITH ":= _your_definition_ ." *). Admitted.
-
-(** After you've defined [s_compile], prove the following to test
-    that it works. *)
-
-Example s_compile1 :
-    s_compile (AMinus (AId X) (AMult (ANum 2) (AId Y)))
-  = [SLoad X; SPush 2; SLoad Y; SMult; SMinus].
-(* FILL IN HERE *) Admitted.
-(** [] *)
-
-(** **** Exercise: 4 stars, advanced (stack_compiler_correct)  *)
-(** Now we'll prove the correctness of the compiler implemented in the
-    previous exercise.  Remember that the specification left
-    unspecified what to do when encountering an [SPlus], [SMinus], or
-    [SMult] instruction if the stack contains less than two
-    elements.  (In order to make your correctness proof easier you
-    might find it helpful to go back and change your implementation!)
-
-    Prove the following theorem.  You will need to start by stating a
-    more general lemma to get a usable induction hypothesis; the main
-    theorem will then be a simple corollary of this lemma. *)
-
-
-Theorem s_compile_correct : forall (st : state) (e : exp),
-  s_execute st [] (s_compile e) = [ aeval st e ].
-Proof.
-  (* FILL IN HERE *) Admitted.
-(** [] *)
-
-(** **** Exercise: 3 stars, optional (short_circuit)  *)
-(** Most modern programming languages use a "short-circuit" evaluation
-    rule for boolean [and]: to evaluate [BAnd b1 b2], first evaluate
-    [b1].  If it evaluates to [false], then the entire [BAnd]
-    expression evaluates to [false] immediately, without evaluating
-    [b2].  Otherwise, [b2] is evaluated to determine the result of the
-    [BAnd] expression.
-
-    Write an alternate version of [beval] that performs short-circuit
-    evaluation of [BAnd] in this manner, and prove that it is
-    equivalent to [beval]. *)
-
-(* FILL IN HERE *)
-(** [] *)
-
-Module BreakImp.
-(** **** Exercise: 4 stars, advanced (break_imp)  *)
-
-(** Imperative languages like C and Java often include a [break] or
-    similar statement for interrupting the execution of loops. In this
-    exercise we consider how to add [break] to Imp.  First, we need to
-    enrich the language of commands with an additional case. *)
-
-Inductive com : Type :=
-  | CSkip : com
-  | CBreak : com               (* <-- new *)
-  | CAss : id -> exp -> com
-  | CSeq : com -> com -> com
-  | CIf : exp -> com -> com -> com
-  | CWhile : exp -> com -> com.
-
-Notation "'SKIP'" :=
-  CSkip.
-Notation "'BREAK'" :=
-  CBreak.
-Notation "x '::=' a" :=
-  (CAss x a) (at level 60).
-Notation "c1 ;; c2" :=
-  (CSeq c1 c2) (at level 80, right associativity).
-Notation "'WHILE' b 'DO' c 'END'" :=
-  (CWhile b c) (at level 80, right associativity).
-Notation "'IFB' c1 'THEN' c2 'ELSE' c3 'FI'" :=
-  (CIf c1 c2 c3) (at level 80, right associativity).
-
-(** Next, we need to define the behavior of [BREAK].  Informally,
-    whenever [BREAK] is executed in a sequence of commands, it stops
-    the execution of that sequence and signals that the innermost
-    enclosing loop should terminate.  (If there aren't any
-    enclosing loops, then the whole program simply terminates.)  The
-    final state should be the same as the one in which the [BREAK]
-    statement was executed.
-
-    One important point is what to do when there are multiple loops
-    enclosing a given [BREAK]. In those cases, [BREAK] should only
-    terminate the _innermost_ loop. Thus, after executing the
-    following...
-
-       X ::= 0;;
-       Y ::= 1;;
-       WHILE 0 <> Y DO
-         WHILE TRUE DO
-           BREAK
-         END;;
-         X ::= 1;;
-         Y ::= Y - 1
-       END
-
-    ... the value of [X] should be [1], and not [0].
-
-    One way of expressing this behavior is to add another parameter to
-    the evaluation relation that specifies whether evaluation of a
-    command executes a [BREAK] statement: *)
-
-Inductive result : Type :=
-  | SContinue : result
-  | SBreak : result.
-
-Reserved Notation "c1 '/' st '\\' s '/' st'"
-                  (at level 40, st, s at level 39).
-
-(** Intuitively, [c / st \\ s / st'] means that, if [c] is started in
-    state [st], then it terminates in state [st'] and either signals
-    that the innermost surrounding loop (or the whole program) should
-    exit immediately ([s = SBreak]) or that execution should continue
-    normally ([s = SContinue]).
-
-    The definition of the "[c / st \\ s / st']" relation is very
-    similar to the one we gave above for the regular evaluation
-    relation ([c / st \\ st']) -- we just need to handle the
-    termination signals appropriately:
-
-    - If the command is [SKIP], then the state doesn't change and
-      execution of any enclosing loop can continue normally.
-
-    - If the command is [BREAK], the state stays unchanged but we
-      signal a [SBreak].
-
-    - If the command is an assignment, then we update the binding for
-      that variable in the state accordingly and signal that execution
-      can continue normally.
-
-    - If the command is of the form [IFB b THEN c1 ELSE c2 FI], then
-      the state is updated as in the original semantics of Imp, except
-      that we also propagate the signal from the execution of
-      whichever branch was taken.
-
-    - If the command is a sequence [c1 ;; c2], we first execute
-      [c1].  If this yields a [SBreak], we skip the execution of [c2]
-      and propagate the [SBreak] signal to the surrounding context;
-      the resulting state is the same as the one obtained by
-      executing [c1] alone. Otherwise, we execute [c2] on the state
-      obtained after executing [c1], and propagate the signal
-      generated there.
-
-    - Finally, for a loop of the form [WHILE b DO c END], the
-      semantics is almost the same as before. The only difference is
-      that, when [b] evaluates to true, we execute [c] and check the
-      signal that it raises.  If that signal is [SContinue], then the
-      execution proceeds as in the original semantics. Otherwise, we
-      stop the execution of the loop, and the resulting state is the
-      same as the one resulting from the execution of the current
-      iteration.  In either case, since [BREAK] only terminates the
-      innermost loop, [WHILE] signals [SContinue]. *)
-
-(** Based on the above description, complete the definition of the
-    [ceval] relation. *)
-
-Inductive ceval : com -> state -> result -> state -> Prop :=
-  | E_Skip : forall st,
-      CSkip / st \\ SContinue / st
-  (* FILL IN HERE *)
-
-  where "c1 '/' st '\\' s '/' st'" := (ceval c1 st s st').
-
-(** Now prove the following properties of your definition of [ceval]: *)
-
-Theorem break_ignore : forall c st st' s,
-     (BREAK;; c) / st \\ s / st' ->
-     st = st'.
-Proof.
-  (* FILL IN HERE *) Admitted.
-
-Theorem while_continue : forall b c st st' s,
-  (WHILE b DO c END) / st \\ s / st' ->
-  s = SContinue.
-Proof.
-  (* FILL IN HERE *) Admitted.
-
-Theorem while_stops_on_break : forall b c st st',
-  beval st b = true ->
-  c / st \\ SBreak / st' ->
-  (WHILE b DO c END) / st \\ SContinue / st'.
-Proof.
-  (* FILL IN HERE *) Admitted.
-(** [] *)
-
-(** **** Exercise: 3 stars, advanced, optional (while_break_true)  *)
-Theorem while_break_true : forall b c st st',
-  (WHILE b DO c END) / st \\ SContinue / st' ->
-  beval st' b = true ->
-  exists st'', c / st'' \\ SBreak / st'.
-Proof.
-(* FILL IN HERE *) Admitted.
-(** [] *)
-
-(** **** Exercise: 4 stars, advanced, optional (ceval_deterministic)  *)
-Theorem ceval_deterministic: forall (c:com) st st1 st2 s1 s2,
-     c / st \\ s1 / st1  ->
-     c / st \\ s2 / st2 ->
-     st1 = st2 /\ s1 = s2.
-Proof.
-  (* FILL IN HERE *) Admitted.
-
-(** [] *)
-End BreakImp.
-
-(** **** Exercise: 4 stars, optional (add_for_loop)  *)
-(** Add C-style [for] loops to the language of commands, update the
-    [ceval] definition to define the semantics of [for] loops, and add
-    cases for [for] loops as needed so that all the proofs in this file
-    are accepted by Coq.
-
-    A [for] loop should be parameterized by (a) a statement executed
-    initially, (b) a test that is run on each iteration of the loop to
-    determine whether the loop should continue, (c) a statement
-    executed at the end of each loop iteration, and (d) a statement
-    that makes up the body of the loop.  (You don't need to worry
-    about making up a concrete Notation for [for] loops, but feel free
-    to play with this too if you like.) *)
-
-(* FILL IN HERE *)
-(** [] *)
-
-(* $Date: 2017-07-04 07:52:33 -0400 (Tue, 04 Jul 2017) $ *)
-
+  
